break memoize up into state and generic parts

Validator/Hedge/Memoize/Memoize.lean
@@ -100,31 +100,3 @@ def Grammar.Memoize.filter [DecidableEq φ] [Hashable φ] [Monad m]
   [MemoizeKatydid m (φ × Ref n)] (G: Grammar n φ) (Φ: φ → α → Bool)
   (xs: List (Hedge α)) : m { xs' // xs' = Grammar.Katydid.filter G Φ xs } :=
   List.filterMemoize (Grammar.Katydid.validate G Φ) (Grammar.Memoize.validate G Φ) xs
-
-def StateMemoize.Grammar.derive.run {φ: Type} [DecidableEq φ] [Hashable φ]
-  (state: memoizeState (φ × Ref n)) (G: Grammar n φ) (Φ: φ → α → Bool) (r: Regex (φ × Ref n)) (node: Node α): Regex (φ × Ref n) :=
-  StateMemoize.run state (Grammar.Memoize.derive G Φ r node)
-
-lemma StateMemoize.Grammar.derive.run_unfold {φ: Type} [DecidableEq φ] [Hashable φ]
-  (state: memoizeState (φ × Ref n)) (G: Grammar n φ) (Φ: φ → α → Bool) (r: Regex (φ × Ref n)) (node: Node α):
-  (StateMemoize.Grammar.derive.run state G Φ r node) = StateMemoize.run state (Grammar.Memoize.derive G Φ r node) :=
-  rfl
-
-theorem StateMemoize.Grammar.derive.run_is_sound [DecidableEq φ] [Hashable φ]
-  (state: memoizeState (φ × Ref n))
-  (Φ: φ → α → Bool) (G: Grammar n φ) (r: Regex (φ × Ref n)) (node: Node α):
-  StateMemoize.Grammar.derive.run state G Φ r node = Grammar.Katydid.derive G Φ r node := by
-  rw [StateMemoize.Grammar.derive.run_unfold]
-  generalize StateMemoize.run state (Grammar.Memoize.derive G Φ r node) = x
-  obtain ⟨dr, hdr⟩ := x
-  simp only
-  rw [hdr]
-
-theorem StateMemoize.Grammar.derive_commutes [DecidableEq φ] [Hashable φ]
-  (state: memoizeState (φ × Ref n))
-  (Φ: φ → α → Prop) [DecidableRel Φ]
-  (G: Grammar n φ) (r: Regex (φ × Ref n)) (node: Node α):
-  Grammar.Rule.denote G Φ (StateMemoize.Grammar.derive.run state G (decideRel Φ) r node)
-  = Lang.derive (Grammar.Rule.denote G Φ r) node := by
-  rw [StateMemoize.Grammar.derive.run_is_sound]
-  rw [<- Grammar.Katydid.derive_commutes]
