Validator/Regex/Memoize/Memoize.lean
@@ -18,17 +18,15 @@ class MemoizeKatydid (m: Type -> Type u) σ [DecidableEq σ] [Hashable σ] where
   leaveM : (a: leaveParam σ) -> m { b: leaveResult a // b = leave a }
 
 instance (m: Type -> Type u) (σ: Type) [DecidableEq σ] [Hashable σ] [Monad m]
-  [DecidableEq (enterParam σ)] [Hashable (enterParam σ)]
   [Memoize (α := enterParam σ) (β := enterResult) enter m]
   [enterState: MonadState (enterMemTable σ) m]
-  [DecidableEq (leaveParam σ)] [Hashable (leaveParam σ)]
   [Memoize (α := leaveParam σ) (β := leaveResult) leave m]
   [leaveState: MonadState (leaveMemTable σ) m]
   : MemoizeKatydid m σ where
   enterM param := MemTable.enter (monadState := enterState) param
   leaveM param := MemTable.leave (monadState := leaveState) param
 
-def Regex.Memoize.derive [Monad m] [DecidableEq σ] [Hashable σ] [MemoizeKatydid m σ]
+def derive [Monad m] [DecidableEq σ] [Hashable σ] [MemoizeKatydid m σ]
   (Φ: σ → Bool) (r: Regex σ): m {dr: Regex σ // dr = Regex.Katydid.derive Φ r } := do
   let ⟨symbols, hsymbols⟩ <- MemoizeKatydid.enterM r
   let ⟨res, hres⟩ <- MemoizeKatydid.leaveM ⟨r, Vector.map Φ symbols⟩
@@ -39,71 +37,10 @@ def Regex.Memoize.derive [Monad m] [DecidableEq σ] [Hashable σ] [MemoizeKatydi
     assumption
   pure (Subtype.mk res h)
 
-abbrev StateMemoize σ [DecidableEq σ] [Hashable σ] := StateT (enterMemTable σ) (StateM (leaveMemTable σ))
-abbrev memoizeState σ [DecidableEq σ] [Hashable σ] := (enterMemTable σ × leaveMemTable σ)
-def memoizeState.init {σ: Type} [DecidableEq σ] [Hashable σ]: memoizeState σ := ((MemTable.init enter), (MemTable.init leave))
-
-def StateMemoize.run {σ: Type} {β: Type} [DecidableEq σ] [Hashable σ]
-  (state: memoizeState σ) (f: StateMemoize σ β): β :=
-  ((StateM.run (StateT.run f state.1) state.2).1).1
-
-def StateMemoize.Regex.derive [DecidableEq σ] [Hashable σ] (Φ: σ → Bool) (r: Regex σ): StateMemoize σ (Regex σ) :=
-  Regex.Memoize.derive Φ r
-
-def StateMemoize.Regex.derive.run {σ: Type} [DecidableEq σ] [Hashable σ]
-  (state: memoizeState σ) (Φ: σ → Bool) (r: Regex σ): Regex σ :=
-  StateMemoize.run state (Regex.Memoize.derive Φ r)
-
-#guard StateMemoize.Regex.derive.run memoizeState.init
-  (· == 'a') (Regex.or (Regex.symbol 'a') (Regex.symbol 'b'))
-  = Regex.or Regex.emptystr Regex.emptyset
-
 def validate [Monad m] [DecidableEq σ] [Hashable σ] [MemoizeKatydid m σ]
   (Φ: σ → α → Bool) (r: Regex σ) (xs: List α): m Bool :=
   null <$> (List.foldlM (fun dr x => Regex.Memoize.derive (flip Φ x) dr) r xs)
 
-def StateMemoize.Regex.validate [DecidableEq σ] [Hashable σ]
-  (Φ: σ → α → Bool) (r: Regex σ) (xs: List α): StateMemoize σ Bool :=
-  Regex.Memoize.validate Φ r xs
-
-def StateMemoize.Regex.validate.run {σ: Type} [DecidableEq σ] [Hashable σ]
-  (state: memoizeState σ) (Φ: σ → α → Bool) (r: Regex σ) (xs: List α): Bool :=
-  StateMemoize.run state (StateMemoize.Regex.validate Φ r xs)
-
-#guard StateMemoize.Regex.validate.run memoizeState.init
-  (· == ·) (Regex.or (Regex.symbol 'a') (Regex.symbol 'b')) ['a']
-  = true
-
 def filter  [Monad m] [DecidableEq σ] [Hashable σ] [MemoizeKatydid m σ]
   (Φ: σ → α → Bool) (r: Regex σ) (xss: List (List α)): m (List (List α)) :=
   List.filterM (validate Φ r) xss
-
-def StateMemoize.Regex.filter [DecidableEq σ] [Hashable σ]
-  (Φ: σ → α → Bool) (r: Regex σ) (xss: List (List α)): StateMemoize σ (List (List α)) :=
-  Regex.Memoize.filter Φ r xss
-
-def StateMemoize.Regex.filter.run [DecidableEq σ] [Hashable σ]
-  (state: memoizeState σ)
-  (Φ: σ → α → Bool) (r: Regex σ) (xss: List (List α)): List (List α) :=
-  StateMemoize.run state (StateMemoize.Regex.filter Φ r xss)
-
-lemma StateMemoize.Regex.derive.run_unfold [DecidableEq σ] [Hashable σ]
-  (state: memoizeState σ) (Φ: σ → Bool) (r: Regex σ):
-  (StateMemoize.Regex.derive.run state Φ r) = StateMemoize.run state (Regex.Memoize.derive Φ r) :=
-  rfl
-
-theorem StateMemoize.Regex.derive.run_is_sound [DecidableEq σ] [Hashable σ]
-  (state: memoizeState σ)
-  (Φ: σ → Bool) (r: Regex σ):
-  StateMemoize.Regex.derive.run state Φ r = Regex.Katydid.derive Φ r := by
-  rw [StateMemoize.Regex.derive.run_unfold]
-  generalize StateMemoize.run state (Regex.Memoize.derive Φ r) = x
-  obtain ⟨dr, hdr⟩ := x
-  simp only
-  rw [hdr]
-
-theorem Regex.StateMemoize.derive_commutes {σ: Type} {α: Type} [DecidableEq σ] [Hashable σ]
-  (state: memoizeState σ) (Φ: σ → α → Prop) [DecidableRel Φ] (r: Regex σ) (a: α):
-  denote Φ (StateMemoize.Regex.derive.run state (flip (decideRel Φ) a) r) = Lang.derive (denote Φ r) a := by
-  rw [StateMemoize.Regex.derive.run_is_sound]
-  rw [<- Regex.Katydid.derive_commutes]
