Validator/Hedge/Memoize.lean
@@ -1,1 +1,2 @@
 import Validator.Hedge.Memoize.Memoize
+import Validator.Hedge.Memoize.StateMemoize
