Validator/Hedge/Memoize/StateMemoize.lean
@@ -1,0 +1,49 @@
+import Mathlib.Tactic.SimpRw
+
+import Validator.Std.Decidable
+import Validator.Std.Hedge
+import Validator.Std.Vec
+
+import Validator.Regex.Lang
+import Validator.Regex.Katydid
+import Validator.Regex.Enter
+import Validator.Regex.Memoize.Memoize
+import Validator.Hedge.Denote
+import Validator.Hedge.Grammar
+import Validator.Hedge.Katydid
+import Validator.Hedge.Lang
+import Validator.Hedge.Denote
+
+import Validator.Hedge.Memoize.Memoize
+
+open Regex.Memoize
+
+namespace Hedge
+
+def StateMemoize.Grammar.derive.run {φ: Type} [DecidableEq φ] [Hashable φ]
+  (state: memoizeState (φ × Ref n)) (G: Grammar n φ) (Φ: φ → α → Bool) (r: Regex (φ × Ref n)) (node: Node α): Regex (φ × Ref n) :=
+  StateMemoize.run state (Grammar.Memoize.derive G Φ r node)
+
+lemma StateMemoize.Grammar.derive.run_unfold {φ: Type} [DecidableEq φ] [Hashable φ]
+  (state: memoizeState (φ × Ref n)) (G: Grammar n φ) (Φ: φ → α → Bool) (r: Regex (φ × Ref n)) (node: Node α):
+  (StateMemoize.Grammar.derive.run state G Φ r node) = StateMemoize.run state (Grammar.Memoize.derive G Φ r node) :=
+  rfl
+
+theorem StateMemoize.Grammar.derive.run_is_sound [DecidableEq φ] [Hashable φ]
+  (state: memoizeState (φ × Ref n))
+  (Φ: φ → α → Bool) (G: Grammar n φ) (r: Regex (φ × Ref n)) (node: Node α):
+  StateMemoize.Grammar.derive.run state G Φ r node = Grammar.Katydid.derive G Φ r node := by
+  rw [StateMemoize.Grammar.derive.run_unfold]
+  generalize StateMemoize.run state (Grammar.Memoize.derive G Φ r node) = x
+  obtain ⟨dr, hdr⟩ := x
+  simp only
+  rw [hdr]
+
+theorem StateMemoize.Grammar.derive_commutes [DecidableEq φ] [Hashable φ]
+  (state: memoizeState (φ × Ref n))
+  (Φ: φ → α → Prop) [DecidableRel Φ]
+  (G: Grammar n φ) (r: Regex (φ × Ref n)) (node: Node α):
+  Grammar.Rule.denote G Φ (StateMemoize.Grammar.derive.run state G (decideRel Φ) r node)
+  = Lang.derive (Grammar.Rule.denote G Φ r) node := by
+  rw [StateMemoize.Grammar.derive.run_is_sound]
+  rw [<- Grammar.Katydid.derive_commutes]
