Validator/Regex/Memoize.lean
@@ -2,3 +2,4 @@ import Validator.Regex.Memoize.Enter
 import Validator.Regex.Memoize.Leave
 import Validator.Regex.Memoize.Memoize
 import Validator.Regex.Memoize.UncurriedDerive
+import Validator.Regex.Memoize.StateMemoize
